src/verilog/AssocMap.v
@@ -1,0 +1,60 @@
+(*
+ * CoqUp: Verified high-level synthesis.
+ * Copyright (C) 2020 Yann Herklotz <yann@yannherklotz.com>
+ *
+ * This program is free software: you can redistribute it and/or modify
+ * it under the terms of the GNU General Public License as published by
+ * the Free Software Foundation, either version 3 of the License, or
+ * (at your option) any later version.
+ *
+ * This program is distributed in the hope that it will be useful,
+ * but WITHOUT ANY WARRANTY; without even the implied warranty of
+ * MERCHANTABILITY or FITNESS FOR A PARTICULAR PURPOSE.  See the
+ * GNU General Public License for more details.
+ *
+ * You should have received a copy of the GNU General Public License
+ * along with this program.  If not, see <https://www.gnu.org/licenses/>.
+ *)
+
+From coqup Require Import Coquplib Value.
+From Coq Require Import FSets.FMapPositive.
+
+Definition reg := positive.
+
+Module AssocMap := PositiveMap.
+
+Module AssocMapExt.
+  Import AssocMap.
+
+  Section Operations.
+
+    Variable elt : Type.
+
+    Definition merge : t elt -> t elt -> t elt := fold (@add elt).
+
+    Definition find_default (a : elt) (k : reg) (m : t elt) : elt :=
+      match find k m with
+      | None => a
+      | Some v => v
+      end.
+
+  End Operations.
+
+End AssocMapExt.
+Import AssocMapExt.
+
+Definition assocmap := AssocMap.t value.
+
+Definition find_assocmap (n : nat) : reg -> assocmap -> value :=
+  find_default value (ZToValue n 0).
+
+Definition empty_assocmap : assocmap := AssocMap.empty value.
+
+Definition merge_assocmap : assocmap -> assocmap -> assocmap := merge value.
+
+Module AssocMapNotation.
+  Notation "a ! b" := (AssocMap.find b a) (at level 1).
+  Notation "a # ( b , c )" := (find_assocmap c b a) (at level 1).
+  Notation "a # b" := (find_assocmap 32 b a) (at level 1).
+  Notation "a ## b" := (List.map (fun c => find_assocmap 32 c a) b) (at level 1).
+End AssocMapNotation.
